Add fixpoint_is_equal axioms and lemmas

wasm-proofs/Wasm-Proof/Host.thy
@@ -1,7 +1,63 @@
 theory Host
-  imports WebAssembly_Dev.Wasm_Ast
+  imports WebAssembly_Dev.Wasm_Ast WebAssembly_Dev.Wasm_Interpreter WebAssembly_Dev.Wasm_Base_Defs coupon
 begin
 
+(* Establish translation between externref and handles *)
+consts to_externref :: "handle \<Rightarrow> host" 
+consts to_handle :: "host \<Rightarrow> handle"
+
+axiomatization where
+  to_externref_to_handle[simp]: "to_externref (to_handle x) = x"
+and
+  to_handle_to_externref[simp]: "to_handle (to_externref y) = y"
+
+definition type0 :: "tf" where 
+  "type0 = Tf [(T_ref T_ext_ref), (T_ref T_ext_ref)] [(T_num T_i32)]"
+
 consts fixpoint_is_equal :: host_func
+
+fun bool_to_i32 :: "bool \<Rightarrow> i32" where
+  "bool_to_i32 False = (I32.int_of_nat 0)"
+| "bool_to_i32 True = (I32.int_of_nat 1)"
+
+lemma i32_one_ne_zero[simp]:
+  "(I32.lift0 1) \<noteq> I32.lift0 0"
+  by transfer simp
+
+lemma bool_to_i32_true:
+  "bool_to_i32 a = (I32.int_of_nat 1) \<longleftrightarrow> a"
+proof
+  assume assms: "bool_to_i32 a = (I32.int_of_nat 1)"
+  show "a"
+  proof (cases "a")
+    case True
+    then show ?thesis by auto
+  next
+    case False
+    then have "bool_to_i32 a = (I32.int_of_nat 0)"  by auto
+    then show ?thesis using assms I32.int_of_nat_def by auto
+  qed
+next
+  assume a
+  then show "bool_to_i32 a = (I32.int_of_nat 1)" by auto
+qed
+
+axiomatization where
+  fixpoint_is_equal_impl:
+  "host_func_apply_impl s type0 fixpoint_is_equal 
+  [(V_ref (ConstRefExtern r1)), (V_ref (ConstRefExtern r2))]
+  = Some (s, [V_num (ConstInt32 (bool_to_i32 (is_equal (to_handle r1) (to_handle r2))))])"
+
+term "ConstInt32 (I32.int_of_nat 1)"
+
+lemma fixpoint_is_equal_correct_handle:
+  "is_equal h1 h2 \<longleftrightarrow> host_func_apply_impl s type0 fixpoint_is_equal 
+  [(V_ref (ConstRefExtern (to_externref h1))), (V_ref (ConstRefExtern (to_externref h2)))] = Some(s, [V_num (ConstInt32 (I32.int_of_nat 1))])"
+  using fixpoint_is_equal_impl bool_to_i32_true by auto
+
+lemma fixpoint_is_equal_correct_externref:
+  "is_equal (to_handle r1) (to_handle r2) \<longleftrightarrow> host_func_apply_impl s type0 fixpoint_is_equal 
+  [(V_ref (ConstRefExtern r1)), (V_ref (ConstRefExtern r2))] = Some(s, [V_num (ConstInt32 (I32.int_of_nat 1))])"
+  using fixpoint_is_equal_impl bool_to_i32_true by auto
 
 end
